src/impl/TLS13.Impl.Server.fsti
@@ -380,6 +380,40 @@ fn process_install_client_handshake_read_keys
                      network_out_bytes
                      app_out_bytes)
 
+fn process_derive_and_install_client_handshake_read_keys
+  (s:server)
+  (network_out:array U8.t)
+  (network_out_len:SZ.t)
+  (app_out:array U8.t)
+  (app_out_len:SZ.t)
+  requires connection_exactly s 'st0 **
+           pts_to network_out 'old_network_out **
+           pts_to app_out 'old_app_out **
+           pure (B.length 'old_network_out == SZ.v network_out_len /\
+                     B.length 'old_app_out == SZ.v app_out_len /\
+                     ST.server_end_to_end_invariant 'st0 /\
+                     'st0.CS.cs_model.CS.model_control ==
+                       CS.ControlHandshaking CS.HsServerHelloSent /\
+                     'st0.CS.cs_model.CS.model_config.CS.config_role ==
+                       CS.ServerEndpoint /\
+                     Some?
+                       'st0.CS.cs_model.CS.model_handshake.CS.hs_keys.CS.ks_handshake_secret)
+  returns resp:ST.server_response
+  ensures exists* st1 network_out_bytes app_out_bytes.
+          connection_exactly s st1 **
+          pts_to network_out network_out_bytes **
+          pts_to app_out app_out_bytes **
+          pure (B.length network_out_bytes == SZ.v network_out_len /\
+                B.length app_out_bytes == SZ.v app_out_len /\
+                ST.server_local_event_end_to_end_correct
+                       'st0
+                       st1
+                       resp
+                       ST.LocalInstallClientHandshakeTrafficKeys
+                       B.empty
+                       network_out_bytes
+                       app_out_bytes)
+
 fn process_client_hello
   (s:server)
   (raw:array U8.t)
